%@+leo-ver=4-thin
%@+node:gcross.20091027203719.1386:@thin FockDarwin.tex
%@@language latex
%\documentclass[onecolumn,amsmath,amssymb,nofootinbib,floatfix]{revtex4}
\documentclass{article}
\usepackage{amsmath,amssymb}

\usepackage{ulem}
\input{notes-prelude.in}

\begin{document}

Consider the case of $N$ bosons in a circular cross-section trap
rotating with angular velocity $\Omega$;  the Hamiltonian for such a
system is given by
$$H = \sum_{i=1}^N \left[\frac{p_{x_i}^2 + p_{y_i}^2 + p_{z_i}^2}{2} - \Omega(x_i
  p_{y_i} - y p_{x_i}) + \frac{\om^2}{2}(x^2+y^2) + \frac{\om_z^2}{2}z^2\right].$$

We define the ladder operators
$$
\begin{aligned}
&a_i:= \sqrt{\frac{\om}{2}}x_i + i\sqrt{\frac{1}{2\om}}p_{x_i},
&a_i^\dagger := \sqrt{\frac{\om}{2}}x_i - i\sqrt{\frac{1}{2\om}}p_{x_i},\\
&b_i:= \sqrt{\frac{\om}{2}}y_i + i\sqrt{\frac{1}{2\om}}p_{y_i},
&b_i^\dagger := \sqrt{\frac{\om}{2}}y_i - i\sqrt{\frac{1}{2\om}}p_{y_i} ,\\
&c_i:= \sqrt{\frac{\om_z}{2}}z_i + i\sqrt{\frac{1}{2\om_z}}p_{z_i},
&c_i^\dagger := \sqrt{\frac{\om_z}{2}}z_i - i\sqrt{\frac{1}{2\om_z}}p_{z_i} ,\\
\end{aligned}
$$
and then observe that using these operators we can re-write our
original Hamiltonian in the form,

$$
\begin{aligned}
H
&= \sum_{i=1}^N \left[\om\paren{a_i^\dagger a_i + b^\dagger b + 1} +  \om_z\paren{c_i^\dagger c_i + \half} - i\Omega\paren{a_i^\dagger b_i - b_i^\dagger a_i}\right],\\
\end{aligned}
$$
To diagonalize this, we let
$$
\begin{aligned}
&\gamma_i := \frac{a_i + i b_i}{\sqrt{2}}, \quad \eta_i := \frac{i a_i + b_i}{\sqrt{2}},
&\Rightarrow\quad a_i = \sqrt{2}(\gamma_i - i \eta_i), \quad b_i = \sqrt{2}(\eta_i - i \gamma_i).
\end{aligned}
$$
Note that
$$
\begin{aligned}
\left[\gamma_i,\gamma_i^\dagger\right] &=
  \frac{\left[a_i,a_i^\dagger\right] +
  \left[ib_i,-ib_i^\dagger\right]}{2} = \frac{1+1}{2} = 1,\\
\left[\eta_i,\eta_i^\dagger\right] &=
  \frac{\left[i a_i,-i a_i^\dagger\right] +
  \left[b_i,b_i^\dagger\right]}{2} = \frac{1+1}{2} = 1,
\end{aligned}
$$
so we see that these new ladder operators satisfy the usual
commutation relations.  Rewriting our Hamiltonian in terms of these
operators, we obtain
$$
\begin{aligned}
H
&=  \sum_{i=1}^N \left\{\om\left[\gamma_i^\dagger\gamma_i + \eta_i^\dagger\eta_i + \half\right] + \om_z\paren{c_i^\dagger c_i + \half}+ \Omega\left[\gamma_i^\dagger\gamma_i - \eta_i^\dagger\eta_i\right]\right\}
\end{aligned}
$$
We now want to examine the angular momentum of eigenstates of the Hamiltonian.
First, we note that the position and momentum operators can be expressed in terms of the new ladder operators as follows:
$$
\begin{aligned}[]
x_i &= \frac{1}{2\sqrt{\om}}[\gamma_i^\dagger + \gamma_i+ i(\eta_i^\dagger-\eta_i)]\\
y_i &= \frac{1}{2\sqrt{\om}}[\eta_i^\dagger + \eta_i+ i(\gamma_i^\dagger-\gamma_i)]\\
p_{x_i} &= i\frac{\sqrt{\om}}{2}[\gamma_i^\dagger - \gamma_i + i(\eta_i^\dagger + \eta_i)]\\
p_{y_i} &=i\frac{\sqrt{\om}}{2}[\eta_i^\dagger - \eta_i + i(\gamma_i^\dagger + \gamma_i)]\\
\end{aligned}
$$
We first shall write the angular momentum operators in terms of the ladder operators:
$$
\begin{aligned}
J_{x_i} &= y_ip_{z_i} - z_ip_{y_i} =+ \sqrt{\frac{}{2m\om}}[\eta_i^\dagger + \eta_i+ i(\gamma_i^\dagger-\gamma_i)] i\sqrt{\frac{\om_z m}{2}}[c_i^\dagger - c_i] -  \sqrt{\frac{}{2m\om_z}}[c_i^\dagger+c_i]  i\sqrt{\frac{\om m}{2}}[\eta_i^\dagger - \eta_i + i(\gamma_i^\dagger + \gamma_i)] \\
&= \frac{}{2}\left\{-\sqrt{\frac{\om_z}{\om}}[(\gamma_i^\dagger-\gamma_i) -i(\eta_i^\dagger + \eta_i)] [c_i^\dagger - c_i] +  \sqrt{\frac{\om}{\om_z}} [ (\gamma_i^\dagger + \gamma_i) -i(\eta_i^\dagger - \eta_i)][c_i^\dagger+c_i] \right\}\\
J_{x_i}^2 &= \frac{^2}{4}\left\{-\sqrt{\frac{\om_z}{\om}}[(\gamma_i^\dagger-\gamma_i) -i(\eta_i^\dagger + \eta_i)] [c_i^\dagger - c_i] +  \sqrt{\frac{\om}{\om_z}} [ (\gamma_i^\dagger + \gamma_i) -i(\eta_i^\dagger - \eta_i)][c_i^\dagger+c_i] \right\}^2\\
\end{aligned}
$$
$$
\begin{aligned}
J_{y_i} &= z_ip_{x_i} - x_ip_{z_i} = - \sqrt{\frac{}{2m\om}}[\gamma_i^\dagger + \gamma_i+ i(\eta_i^\dagger-\eta_i)]i\sqrt{\frac{\om_z m}{2}}[c_i^\dagger - c_i] + i\sqrt{\frac{\om m}{2}}[\gamma_i^\dagger - \gamma_i + i(\eta_i^\dagger + \eta_i)]\sqrt{\frac{}{2m\om_z}}[c_i^\dagger+c_i]\\
&= \frac{}{2}\left\{\sqrt{\frac{\om_z}{\om}}[(\eta_i^\dagger-\eta_i) - i(\gamma_i^\dagger + \gamma_i)][c_i^\dagger - c_i] - \frac{}{2}[(\eta_i^\dagger + \eta_i)-i(\gamma_i^\dagger - \gamma_i)][c_i^\dagger+c_i]\right\}\\
J_{z_i}&=\eta_i^\dagger\eta_i - \gamma_i^\dagger\gamma_i\\
\end{aligned}
$$
Observe that $[J_{z_i},H]=0$, so that the $z$ component of angular momentum and the energy can be known simultaneously.  Furthermore, all states which are eigenstates of $\gamma_i^\dagger\gamma_i$ and $\eta_i^\dagger\eta_i$ are also eigenstates of $J_z$.
Now let us consider $J_i^2$, so that we now need to calculate
\end{document}
%@-node:gcross.20091027203719.1386:@thin FockDarwin.tex
%@-leo
